Got all the way through fieldlist.v

floyd/fieldlist.v
@@ -5,52 +5,75 @@ Import compcert.lib.Maps.
 Arguments align !n !amount / .
 Arguments Z.max !n !m / .
 
-Definition plain_member (m: member) : Prop :=
- match m with Member_plain _ _ => True | _ => False end.
+Fixpoint plain_members (m: members) : option (list (ident*type)) :=
+ match m with
+ | Member_plain i t :: m' => match plain_members m' with
+                                             | Some l => Some ((i,t)::l)
+                                             | None => None
+                                             end
+ | _ :: _ => None
+ | nil => Some nil
+ end.
 
-Definition plain_members : members->Prop := Forall plain_member.
+Fixpoint field_type' i (m: list (ident*type)) : option type :=
+ match m with
+ | (j,t)::m' => if ident_eq i j then Some t else field_type' i m'
+ | nil => None
+ end.
 
-Definition field_type i m :=
-  match Ctypes.field_type i m with
-  | Errors.OK t => t
-  | _ => Tvoid
+Fixpoint field_type i (m: list (ident*type)) : type :=
+ match m with
+ | (j,t)::m' => if ident_eq i j then t else field_type i m'
+ | nil => Tvoid
+ end.
+
+Lemma field_type_field_type': forall i m,
+  field_type i m = match field_type' i m with Some t => t | None => Tvoid end.
+Proof.
+induction m as [| [? ? ]]; simpl; intros; auto. if_tac; auto.
+Qed.
+
+Fixpoint field_offset_rec (env: composite_env) (id: ident) (fld: list (ident*type)) (pos: Z)
+                          {struct fld} : Z :=
+  match fld with
+  | nil => -1
+  | (id', t) :: fld' =>
+      if ident_eq id id'
+      then align pos (@Ctypes.alignof env t)
+      else field_offset_rec env id fld' (align pos (@Ctypes.alignof env t) + @Ctypes.sizeof env t)
   end.
 
-Definition field_offset env i m :=
-  match Ctypes.field_offset env i m with
-  | Errors.OK (ofs, Full) => ofs
-  | _ => 0
-  end.
+Definition field_offset env (i: ident) (m: list (ident*type)) : Z   := field_offset_rec env i m 0.
 
 Fixpoint field_offset_next_rec (env:composite_env) i m ofs sz :=
   match m with
   | nil => 0
-  | m1 :: m0 =>
+  | (i0, t0) :: m0 =>
     match m0 with
     | nil => sz
-    | m2 :: _ =>
-      if ident_eq i (name_member m1)
-      then align (ofs + @Ctypes.sizeof env (type_member m1)) (@Ctypes.alignof env (type_member m2))
-      else field_offset_next_rec env i m0 (align (ofs + @Ctypes.sizeof env (type_member m1)) (@Ctypes.alignof env (type_member m2))) sz
+    | (_, t1) :: _ =>
+      if ident_eq i i0
+      then align (ofs + @Ctypes.sizeof env t0) (@Ctypes.alignof env t1)
+      else field_offset_next_rec env i m0 (align (ofs + @Ctypes.sizeof env t0) (@Ctypes.alignof env t1)) sz
     end
   end.
 
 Definition field_offset_next (env:composite_env) i m sz := field_offset_next_rec env i m 0 sz.
 
-Definition in_members i (m: members): Prop :=
-  In i (map name_member m).
+Definition in_members i (m: list (ident*type)): Prop :=
+  In i (map fst m).
 
-Definition members_no_replicate (m: members) : bool :=
-  compute_list_norepet (map name_member m).
+Definition members_no_replicate (m: list (ident*type)) : bool :=
+  compute_list_norepet (map fst m).
 
-Definition compute_in_members id (m: members): bool :=
-  id_in_list id (map name_member m).
+Definition compute_in_members id (m: list (ident*type)): bool :=
+  id_in_list id (map fst m).
 
 Lemma compute_in_members_true_iff: forall i m, compute_in_members i m = true <-> in_members i m.
 Proof.
   intros.
   unfold compute_in_members.
-  destruct (id_in_list i (map name_member m)) eqn:HH;
+  destruct (id_in_list i (map fst m)) eqn:HH;
   [apply id_in_list_true in HH | apply id_in_list_false in HH].
   + unfold in_members.
     tauto.
@@ -79,70 +102,80 @@ Proof.
 Qed.
 
 Lemma in_members_field_type: forall i m,
-  plain_members m ->
   in_members i m ->
-  In (Member_plain i (field_type i m)) m.
+  In (i, field_type i m) m.
 Proof.
-  unfold members_no_replicate, field_type.
   intros.
-  induction m as [| [|]]; [ | inv H; specialize (IHm H4) .. ].
-  - contradiction H0.
-  -  simpl in *. destruct H0.
-     + subst. left. rewrite if_true by auto. auto. 
-     + if_tac. subst; auto. right. apply IHm; auto.
-  - contradiction.
+  unfold field_type.
+  induction m as [|[i0 t0] m].
+  + inversion H.
+  + unfold in_members in H; simpl in H.
+    destruct (ident_eq i0 i).
+    - subst.
+      simpl.
+      if_tac; [| congruence].
+      left. auto.
+    - simpl.
+      right.
+      destruct H; [congruence |].
+      specialize (IHm H).
+      if_tac; [congruence |].
+      exact IHm.
 Qed.
 
-Lemma field_offset_field_type_match: forall cenv i m,
-  plain_members m ->
-  match Ctypes.field_offset cenv i m, Ctypes.field_type i m with
-  | Errors.OK (_, Full), Errors.OK _ => True
-  | Errors.Error _, Errors.Error _ => True
-  | _, _ => False
+Lemma field_offset_field_type_match': forall cenv i m,
+  match field_offset cenv i m, field_type' i m with
+  | Zneg _, None => True
+  | Zneg _, Some _ => False 
+  | _, Some _ => True
+  | _, None => False
   end.
 Proof.
   intros.
-  unfold Ctypes.field_offset.
-  remember 0 as pos; clear Heqpos.
-  revert pos; induction m; intros.
+  unfold field_offset.
+  set (pos:=0). assert (0 <= pos) by lia. clearbody pos.
+  revert pos H; induction m as [| [? ?] ?]; intros.
   + simpl. auto.
-  + inv H. specialize (IHm H3).
-      simpl. if_tac. subst i.
-      destruct a; simpl. auto.
-      inv H2.
-      apply IHm.
+  + simpl.
+        pose proof (align_le pos _ (Ctypes.alignof_pos t)).
+        if_tac. subst.
+    - destruct (align pos (Ctypes.alignof t)); auto; lia.
+    - apply IHm. pose proof (Ctypes.sizeof_pos t). lia.
+Qed.
+
+Lemma field_offset_field_type_match: forall cenv i m,
+  match zlt (field_offset cenv i m) 0, field_type' i m with
+  | left _, None => True
+  | left _, Some _ => False 
+  | right _, Some _ => True
+  | right _, None => False
+  end.
+Proof.
+  intros.
+  pose proof (field_offset_field_type_match' cenv i m).
+  destruct (field_offset cenv i m); auto.
 Qed.
 
 Lemma field_type_in_members: forall i m,
-  match Ctypes.field_type i m with
-  | Errors.Error _ => ~ in_members i m
+  match field_type' i m with
+  | None => ~ in_members i m
   | _ => in_members i m
   end.
 Proof.
   intros.
   unfold in_members.
-  induction m.
+  induction m as [| [i0 t0] m].
   + simpl; tauto.
   + simpl.
-     if_tac.
+    destruct (ident_eq i i0).
     - left; subst; auto.
-    - destruct (Ctypes.field_type i m).
+    - destruct (field_type' i m).
       * right; auto.
       * intro HH; destruct HH; [congruence | tauto].
 Qed.
 
 Section COMPOSITE_ENV.
 Context {cs: compspecs}.
-
-Ltac solve_field_offset_type i m PLAIN :=
-  let H := fresh "H" in
-  let Hty := fresh "H" in
-  let Hofs := fresh "H" in
-  let t := fresh "t" in
-  let ofs := fresh "ofs" in
-  assert (H := field_offset_field_type_match cenv_cs i m PLAIN);
-  destruct (Ctypes.field_offset cenv_cs i m) as [[ofs [|]]|?] eqn:Hofs, (Ctypes.field_type i m) as [t|?] eqn:Hty;
-   [clear H | inversion H | inversion H | inversion H | inversion H | clear H ].
 
 Lemma complete_legal_cosu_member: forall (cenv : composite_env) (id : ident) (t : type) (m : members),
   In (Member_plain id t) m -> @composite_complete_legal_cosu_type cenv m = true -> @complete_legal_cosu_type cenv t = true.
@@ -159,216 +192,50 @@ Proof.
       rewrite andb_true_iff in H0; tauto.
 Qed.         
 
-Lemma complete_legal_cosu_type_field_type: forall id i
-  (PLAIN: plain_members (co_members (get_co id))),
-  in_members i (co_members (get_co id)) ->
-  complete_legal_cosu_type (field_type i (co_members (get_co id))) = true.
+Lemma in_plain_members:
+  forall m m'
+  (PLAIN: plain_members m = Some m'),
+   forall i t,
+  In (Member_plain i t) m <-> In (i,t) m'.
+Proof.
+ induction m; destruct m'; simpl; intros; try discriminate.
+ tauto.
+ destruct a.
+ destruct (plain_members m); discriminate.
+ discriminate.
+ destruct a.
+ destruct (plain_members m). inv PLAIN.
+ specialize (IHm m' (eq_refl _)).
+ rewrite <- IHm.
+ split; intros [?|?]; auto. inv H; auto. inv H; auto. inv PLAIN. inv PLAIN.
+Qed.
+
+Lemma complete_legal_cosu_type_field_type: forall m id
+  (PLAIN: plain_members (co_members (get_co id)) = Some m)
+  i,
+  in_members i m ->
+  complete_legal_cosu_type (field_type i m) = true.
 Proof.
   unfold get_co.
   intros.
   destruct (cenv_cs ! id) as [co |] eqn:CO.
-  + apply in_members_field_type in H; auto.
+  + apply in_members_field_type in H.
     pose proof cenv_legal_su _ _ CO.
-    eapply complete_legal_cosu_member; eauto.
-  + inversion H.
+    apply complete_legal_cosu_member with i (co_members co); eauto.
+    apply <- in_plain_members; eauto.
+  + simpl in PLAIN. inv PLAIN. inversion H.
 Qed.
 
-Lemma align_compatible_rec_Tstruct_inv': forall id
-  (PLAIN: plain_members (co_members (get_co id)))
-  a ofs,
-  align_compatible_rec cenv_cs (Tstruct id a) ofs ->
-  forall i,
-  in_members i (co_members (get_co id)) ->
-  align_compatible_rec cenv_cs (field_type i (co_members (get_co id)))
-    (ofs + field_offset cenv_cs i (co_members (get_co id))).
+Lemma plain_members_field_type:
+  forall m m' 
+  (PLAIN: plain_members m = Some m')
+  i, in_members i m' -> Ctypes.field_type i m = Errors.OK (field_type i m').
 Proof.
-  unfold get_co.
-  intros.
-  destruct (cenv_cs ! id) as [co |] eqn:CO.
-  + eapply align_compatible_rec_Tstruct_inv with (i0 := i); try eassumption.
-    - unfold field_type.
-      induction (co_members co).
-      * inv H0.
-      * simpl; if_tac; auto.
-        apply IHm. inv PLAIN; auto.
-        destruct H0; [simpl in H0; congruence | auto].
-    - unfold field_offset, Ctypes.field_offset.
-      generalize 0 at 1 2.
-      induction (co_members co); intros.
-      * inv H0.
-      * unfold field_offset_rec; fold field_offset_rec.
-        inv PLAIN. destruct a0; try contradiction. simpl.
-        if_tac; auto.
-        apply IHm; auto.
-        destruct H0; [simpl in H0; congruence | auto].
-  + inv H0.
-Qed.
-
-Lemma align_compatible_rec_Tunion_inv': forall id a ofs,
-  align_compatible_rec cenv_cs (Tunion id a) ofs ->
-  forall i,
-  in_members i (co_members (get_co id)) ->
-  align_compatible_rec cenv_cs (field_type i (co_members (get_co id))) ofs.
-Proof.
-  unfold get_co.
-  intros.
-  destruct (cenv_cs ! id) as [co |] eqn:CO.
-  + eapply align_compatible_rec_Tunion_inv with (i0 := i); try eassumption.
-    unfold field_type.
-    induction (co_members co).
-    - inv H0.
-    - simpl; if_tac; auto.
-      apply IHm.
-      destruct H0; [simpl in H0; congruence | auto].
-  + inv H0.
-Qed.
-
-Lemma field_offset_aligned: forall i m,
-  (alignof (field_type i m) | field_offset cenv_cs i m).
-Proof.
-  intros.
- unfold field_offset. unfold field_type.
-  destruct (Ctypes.field_offset cenv_cs i m) as [[? [|]]|] eqn:?H.
-  destruct (Ctypes.field_type i m) eqn:?H.
- apply (field_offset_aligned cenv_cs i m _ _ H H0).
- apply Z.divide_1_l.
- apply Z.divide_0_r.
- apply Z.divide_0_r.
-Qed.
-
-Lemma alignof_composite_hd_divide: forall m1 m
-  (PLAIN: plain_members (m1::m)),
-  (alignof (type_member m1) | alignof_composite cenv_cs (m1 :: m)).
-Proof.
-  intros.
-  inv PLAIN.
-  destruct (alignof_composite_two_p cenv_cs (m1 :: m)) as [M H0].
-  destruct m1; inv H1.
-  simpl.
-  destruct (alignof_two_p t) as [N H].
-  assert (alignof t <= alignof_composite cenv_cs (Member_plain id t :: m)) by apply Z.le_max_l.
-  fold (alignof t) in H.
-  rewrite H in *.
-  simpl in *.
-  rewrite H0 in *.
-  exact (power_nat_divide N M H1).
-Qed.
-
-Lemma alignof_composite_tl_divide: forall m1 m
-  (PLAIN: plain_members (m1::m)),
-   (alignof_composite cenv_cs m | alignof_composite cenv_cs (m1 :: m)).
-Proof.
-  intros.
-  destruct (alignof_composite_two_p cenv_cs m) as [N ?].
-  destruct (alignof_composite_two_p cenv_cs (m1 :: m)) as [M ?].
-  inv PLAIN. destruct m1; inv H3.
-  assert (alignof_composite cenv_cs m <= alignof_composite cenv_cs (Member_plain id t :: m)) by (apply Z.le_max_r).
-  rewrite H in *.
-  rewrite H0 in *.
-  exact (power_nat_divide N M H1).
-Qed.
-
-Lemma alignof_field_type_divide_alignof: forall i m
-  (PLAIN: plain_members m),
-  in_members i m ->
-  (alignof (field_type i m) | alignof_composite cenv_cs m).
-Proof.
-  intros.
-  unfold field_type.
-  induction m. 
-  + inversion H.
-  + unfold in_members in H; simpl in H.
-    simpl Ctypes.field_type.
-    if_tac.
-    - apply alignof_composite_hd_divide; auto.
-    - eapply Z.divide_trans.
-      * inv PLAIN. apply IHm; auto.
-        destruct H; [congruence | auto].
-      * apply alignof_composite_tl_divide; auto.
-Qed.
-
-(* if sizeof Tvoid = 0, this lemma can be nicer. *)
-Lemma field_offset_in_range: forall i m
-  (PLAIN: plain_members m),
-  in_members i m ->
-  0 <= field_offset cenv_cs i m /\ field_offset cenv_cs i m + sizeof (field_type i m) <= sizeof_struct cenv_cs m.
-Proof.
-  intros.
-  unfold field_offset, field_type.
-  solve_field_offset_type i m PLAIN.
-  + eapply field_offset_in_range; eauto.
-  + pose proof field_type_in_members i m.
-    rewrite H1 in H0.
-    tauto.
-Qed.
-
-(* if sizeof Tvoid = 0, this lemma can be nicer. *)
-Lemma sizeof_union_in_members: forall i m,
-  in_members i m ->
-  sizeof (field_type i m) <= sizeof_union cenv_cs m.
-(* field_offset2_in_range union's version *)
-Proof.
-  intros.
-  unfold in_members in H.
-  unfold field_type.
-  induction m.
-  + inversion H.
-  + simpl.
-    destruct (ident_eq i (name_member a)).
-    - apply Z.le_max_l.
-    - simpl in H; destruct H; [congruence |].
-     specialize (IHm H).
-     fold (sizeof (type_member a)).
-     pose proof Z.le_max_r (sizeof (type_member a)) (sizeof_union cenv_cs m).
-     lia.
-Qed.
-
-(* if sizeof Tvoid = 0, this lemma can be nicer. *)
-Lemma field_offset_no_overlap:
-  forall i1 i2 m
-  (PLAIN: plain_members m),
-  i1 <> i2 ->
-  in_members i1 m ->
-  in_members i2 m ->
-  field_offset cenv_cs i1 m + sizeof (field_type i1 m) <= field_offset cenv_cs i2 m \/
-  field_offset cenv_cs i2 m + sizeof (field_type i2 m) <= field_offset cenv_cs i1 m.
-Proof.
-  intros.
-  unfold field_offset, field_type.
-  pose proof field_type_in_members i1 m.
-  pose proof field_type_in_members i2 m.
-  solve_field_offset_type i1 m PLAIN;
-  solve_field_offset_type i2 m PLAIN; try tauto.
- pose proof (field_offset_no_overlap _ _ _ _ _ _ _ _ _ _ H6 H5 H8 H7 H).
-  unfold layout_start, layout_width, bitsizeof in H4. unfold sizeof. lia.
-Qed.
-
-Lemma not_in_members_field_type: forall i m,
-  ~ in_members i m ->
-  field_type i m = Tvoid.
-Proof.
-  unfold in_members, field_type.
-  intros.
-  induction m.
-  + reflexivity.
-  + simpl in H.
-    simpl.
-    destruct (ident_eq i (name_member a)) as [HH | HH]; pose proof (@eq_sym ident i (name_member a)); tauto.
-Qed.
-
-Lemma not_in_members_field_offset: forall i m,
-  ~ in_members i m ->
-  field_offset cenv_cs i m = 0.
-Proof.
-  unfold in_members, field_offset, Ctypes.field_offset.
-  intros.
-  generalize 0 at 1.
-  induction m; intros.
-  + reflexivity.
-  + simpl in H.
-    simpl.
-    destruct (ident_eq i _) as [HH | HH]; pose proof (@eq_sym ident i (name_member a)); [tauto |].
-    apply IHm. tauto.
+ induction m as [|[|]]; destruct m'; simpl; intros; inv PLAIN. 
+ inv H. inv H.
+ destruct (plain_members m) eqn:?H; inv H1.
+ if_tac. auto.
+ inv H. simpl in H1; congruence. apply IHm; auto.
 Qed.
 
 Lemma align_bitalign: (* copied from veric/align_mem.v *)
@@ -401,60 +268,344 @@ rewrite Z.div_add_l by lia.
 reflexivity.
 Qed.
 
-Lemma field_offset_next_in_range: forall i m sz
-  (PLAIN: plain_members m),
+Lemma plain_members_field_offset:
+  forall m m' 
+  (PLAIN: plain_members m = Some m')
+  env i, in_members i m' -> Ctypes.field_offset env i m = Errors.OK (field_offset env i m', Full).
+Proof.
+ unfold field_offset, Ctypes.field_offset.
+ intros.
+ change 0 with (0*8) at 1.
+ generalize 0. revert m' PLAIN H.
+ induction m as [|[|]]; destruct m'; simpl; intros; inv PLAIN. 
+ inv H. inv H.
+ destruct (plain_members m) eqn:?H; inv H1.
+ if_tac.
+ f_equal. f_equal.
+ unfold bitalignof.
+ symmetry.
+ apply align_bitalign.
+ apply Ctypes.alignof_pos.
+ inv H. simpl in H1; congruence. 
+ rewrite <- (IHm _ (eq_refl _) H2); clear IHm.
+ f_equal. unfold bitalignof, bitsizeof.
+ symmetry.
+ clear.
+ pose proof (Ctypes.alignof_pos t).
+ pose proof (Ctypes.sizeof_pos t).
+ rewrite align_bitalign by auto.
+ forget (Ctypes.alignof t) as a.
+ forget (Ctypes.sizeof t) as s.
+ unfold align.
+ replace (z*8+a*8-1) with (z*8-1+1*(a*8)) by lia.
+ rewrite !Z.div_add by lia.
+ forget (z*8-1) as u.
+ rewrite Z.mul_add_distr_r.
+ f_equal. rewrite Z.mul_assoc.
+ rewrite Z_div_mult by computable.
+ f_equal.
+Qed.
+
+Lemma align_compatible_rec_Tstruct_inv': forall m id
+  (PLAIN: plain_members (co_members (get_co id)) = Some m)
+  a ofs,
+  align_compatible_rec cenv_cs (Tstruct id a) ofs ->
+  forall i,
   in_members i m ->
-  sizeof_struct cenv_cs m <= sz ->
+  align_compatible_rec cenv_cs (field_type i m)
+    (ofs + field_offset cenv_cs i m).
+Proof.
+  unfold get_co.
+  intros.
+  destruct (cenv_cs ! id) as [co |] eqn:CO.
+  + inv H. inv H1.
+      inversion2 CO H3.
+      apply (H5 i (field_type i m) (field_offset cenv_cs i m)); clear H5.
+      apply plain_members_field_type; auto.
+      apply plain_members_field_offset; auto.
+  + inv PLAIN. inv H0.
+Qed.
+
+Lemma align_compatible_rec_Tunion_inv': forall m id
+  (PLAIN: plain_members (co_members (get_co id)) = Some m)
+  a ofs,
+  align_compatible_rec cenv_cs (Tunion id a) ofs ->
+  forall i,
+  in_members i m ->
+  align_compatible_rec cenv_cs (field_type i m) ofs.
+Proof.
+  unfold get_co.
+  intros.
+  destruct (cenv_cs ! id) as [co |] eqn:CO.
+  + inv H. inv H1.
+      inversion2 CO H3.
+      apply (H5 i (field_type i m)); clear H5.
+      apply plain_members_field_type; auto.
+  + inv PLAIN. inv H0.
+Qed.
+
+Lemma field_offset_aligned: forall i m,
+  (alignof (field_type i m) | field_offset cenv_cs i m).
+Proof.
+ intros.
+ unfold field_offset.
+ generalize 0 as pos.
+ induction m as [| [? ?]]; simpl; intros.
+ apply Z.divide_1_l.
+ if_tac.
+ apply align_divides. apply alignof_pos.
+ apply IHm.
+Qed.
+
+Fixpoint alignof_composite (env: composite_env) (m: list (ident*type)) : Z :=
+  match m with
+  | nil => 1
+  | (id, t) :: m' => Z.max (@Ctypes.alignof env t) (alignof_composite env m')
+  end.
+
+Lemma alignof_composite_two_p:
+  forall env m, exists n, alignof_composite env m = two_power_nat n.
+Proof.
+  induction m as [|[id t]]; simpl.
+- exists 0%nat; auto.
+- apply Z.max_case; auto. apply alignof_two_p.
+Qed.
+
+Lemma alignof_composite_pos:
+  forall env m a, align_attr a (alignof_composite env m) > 0.
+Proof.
+  intros.
+  exploit align_attr_two_p. apply (alignof_composite_two_p env m).
+  instantiate (1 := a). intros [n EQ].
+  rewrite EQ; apply two_power_nat_pos.
+Qed.
+
+Lemma alignof_composite_hd_divide: forall i t m, (alignof t | alignof_composite cenv_cs ((i, t) :: m)).
+Proof.
+  intros.
+  destruct (alignof_two_p t) as [N ?].
+  destruct (alignof_composite_two_p cenv_cs ((i, t) :: m)) as [M ?].
+  assert (alignof t <= alignof_composite cenv_cs ((i,t)::m)) by (apply Z.le_max_l).
+  fold (alignof t) in H.
+  rewrite H in *.
+  rewrite H0 in *.
+  exact (power_nat_divide N M H1).
+Qed.
+
+Lemma alignof_composite_tl_divide: forall i t m, (alignof_composite cenv_cs m | alignof_composite cenv_cs ((i, t) :: m)).
+Proof.
+  intros.
+  destruct (alignof_composite_two_p cenv_cs m) as [N ?].
+  destruct (alignof_composite_two_p cenv_cs ((i, t) :: m)) as [M ?].
+  assert (alignof_composite cenv_cs m <= alignof_composite cenv_cs ((i, t) :: m)) by (apply Z.le_max_r).
+  rewrite H in *.
+  rewrite H0 in *.
+  exact (power_nat_divide N M H1).
+Qed.
+
+Lemma alignof_field_type_divide_alignof: forall i m,
+  in_members i m ->
+  (alignof (field_type i m) | alignof_composite cenv_cs m).
+Proof.
+  intros.
+  unfold field_type.
+  induction m as [| [i0 t0] m].
+  + inversion H.
+  + unfold in_members in H; simpl in H.
+    simpl Ctypes.field_type.
+    if_tac.
+    - apply alignof_composite_hd_divide.
+    - eapply Z.divide_trans.
+      * apply IHm.
+        destruct H; [congruence | auto].
+      * apply alignof_composite_tl_divide.
+Qed.
+
+Fixpoint sizeof_struct (env: composite_env) (cur: Z) (m: list(ident*type)) : Z :=
+  match m with
+  | nil => cur
+  | (id, t) :: m' => sizeof_struct env (align cur (@Ctypes.alignof env t) + @Ctypes.sizeof env t) m'
+  end.
+
+Fixpoint sizeof_union (env: composite_env) (m: list(ident*type)) : Z :=
+  match m with
+  | nil => 0
+  | (id, t) :: m' => Z.max (@Ctypes.sizeof env t) (sizeof_union env m')
+  end.
+
+Ltac solve_field_offset_type i m :=
+  let H := fresh "H" in
+  let Hty := fresh "H" in
+  let Hofs := fresh "H" in
+  let t := fresh "t" in
+  let ofs := fresh "ofs" in
+  pose proof field_offset_field_type_match cenv_cs i m;
+  destruct (Ctypes.field_offset cenv_cs i m) as [ofs|?] eqn:Hofs, (Ctypes.field_type i m) as [t|?] eqn:Hty;
+    [clear H | inversion H | inversion H | clear H].
+
+Lemma sizeof_struct_incr:
+  forall env m cur, cur <= sizeof_struct env cur m.
+Proof.
+  induction m as [|[id t]]; simpl; intros.
+- lia.
+- apply Z.le_trans with (align cur (@Ctypes.alignof env t)).
+  apply align_le. apply Ctypes.alignof_pos.
+  apply Z.le_trans with (align cur (@Ctypes.alignof env t) + @Ctypes.sizeof env t).
+  generalize (@Ctypes.sizeof_pos env t); lia.
+  apply IHm.
+Qed.
+
+
+Lemma field_offset_rec_in_range:
+  forall env id ofs ty fld pos,
+  0 <= ofs ->
+  field_offset_rec env id fld pos = ofs -> field_type id fld = ty ->
+  pos <= ofs /\ ofs + @Ctypes.sizeof env ty <= sizeof_struct env pos fld.
+Proof.
+  intros until ty. induction fld as [|[i t]]; simpl; intros.
+- lia.
+- destruct (ident_eq id i).
+   subst. split.
+  apply align_le. apply Ctypes.alignof_pos. apply sizeof_struct_incr.
+  exploit IHfld; eauto. intros [A B]. split; auto.
+  eapply Z.le_trans; try apply A. apply Z.le_trans with (align pos (@Ctypes.alignof env t)).
+  apply align_le. apply Ctypes.alignof_pos. generalize (@Ctypes.sizeof_pos env t). lia.
+Qed.
+
+Lemma in_members_field_offset_pos:
+  forall env i m,
+  in_members i m -> 0 <= field_offset env i m.
+Proof.
+ intros.
+ unfold field_offset.
+ set (pos:=0) at 2.
+ assert (0 <= pos) by lia.
+ clearbody pos.
+ revert pos H0; induction m as [|[??]]; simpl; intros. inv H.
+ if_tac. subst. eapply Z.le_trans. apply H0.
+ apply align_le. apply Ctypes.alignof_pos.
+ destruct H. simpl in H; subst; contradiction. apply IHm; auto.
+ pose proof (Ctypes.alignof_pos t). pose proof (Ctypes.sizeof_pos t).
+ apply Z.le_trans with (align pos (Ctypes.alignof t)); try lia.
+ eapply Z.le_trans. apply H0.
+ apply align_le; auto.
+Qed.
+
+(* if sizeof Tvoid = 0, this lemma can be nicer. *)
+Lemma field_offset_in_range: forall i m,
+  in_members i m ->
+  0 <= field_offset cenv_cs i m /\ field_offset cenv_cs i m + sizeof (field_type i m) <= sizeof_struct cenv_cs 0 m.
+Proof.
+  intros.
+  pose proof (in_members_field_offset_pos cenv_cs i m H).
+  split; auto.
+  apply (field_offset_rec_in_range cenv_cs i (field_offset_rec cenv_cs i m 0) (field_type i m) m 0); auto.
+Qed.
+
+(* if sizeof Tvoid = 0, this lemma can be nicer. *)
+Lemma sizeof_union_in_members: forall i m,
+  in_members i m ->
+  sizeof (field_type i m) <= sizeof_union cenv_cs m.
+(* field_offset2_in_range union's version *)
+Proof.
+  intros.
+  unfold in_members in H.
+  unfold field_type.
+  induction m as [|[i0 t0] m].
+  + inversion H.
+  + simpl.
+    destruct (ident_eq i i0).
+    - apply Z.le_max_l.
+    - simpl in H; destruct H; [congruence |].
+     specialize (IHm H).
+     fold (sizeof t0).
+     pose proof Z.le_max_r (sizeof t0) (sizeof_union cenv_cs m).
+     lia.
+Qed.
+
+Lemma field_offset_no_overlap':
+  forall env id1 ofs1 ty1 id2 ofs2 ty2 fld,
+  0 <= ofs1 -> 0 <= ofs2 ->
+  field_offset env id1 fld = ofs1 -> field_type id1 fld = ty1 ->
+  field_offset env id2 fld = ofs2 -> field_type id2 fld = ty2 ->
+  id1 <> id2 ->
+  ofs1 + @Ctypes.sizeof env ty1 <= ofs2 \/ ofs2 + @Ctypes.sizeof env ty2 <= ofs1.
+Proof.
+  intros until fld. intros G1 G2. unfold field_offset. generalize 0 as pos.
+  induction fld as [|[i t]]; simpl; intros.
+- lia.
+- destruct (ident_eq id1 i); destruct (ident_eq id2 i).
++ congruence.
++ subst. 
+  exploit field_offset_rec_in_range. apply G2. reflexivity. reflexivity. tauto.
++ subst.
+  exploit field_offset_rec_in_range. apply G1. reflexivity. reflexivity. tauto.
++ eapply IHfld; eauto.
+Qed.
+
+(* if sizeof Tvoid = 0, this lemma can be nicer. *)
+Lemma field_offset_no_overlap:
+  forall i1 i2 m,
+  i1 <> i2 ->
+  in_members i1 m ->
+  in_members i2 m ->
+  field_offset cenv_cs i1 m + sizeof (field_type i1 m) <= field_offset cenv_cs i2 m \/
+  field_offset cenv_cs i2 m + sizeof (field_type i2 m) <= field_offset cenv_cs i1 m.
+Proof.
+  intros.
+  eapply field_offset_no_overlap'; eauto.
+  apply in_members_field_offset_pos; auto.
+  apply in_members_field_offset_pos; auto.
+Qed.
+
+Lemma not_in_members_field_type: forall i m,
+  ~ in_members i m ->
+  field_type i m = Tvoid.
+Proof.
+  unfold in_members, field_type.
+  intros.
+  induction m as [| [i0 t0] m].
+  + reflexivity.
+  + simpl in H.
+    simpl.
+    destruct (ident_eq i i0) as [HH | HH]; pose proof (@eq_sym ident i i0); tauto.
+Qed.
+
+Lemma not_in_members_field_offset: forall i m,
+  ~ in_members i m ->
+  field_offset cenv_cs i m = -1.
+Proof.
+  unfold in_members, field_offset, Ctypes.field_offset.
+  intros.
+  generalize 0 at 1.
+  induction m as [| [i0 t0] m]; intros.
+  + reflexivity.
+  + simpl in H.
+    simpl.
+    destruct (ident_eq i i0) as [HH | HH]; pose proof (@eq_sym ident i i0); [tauto |].
+    apply IHm. tauto.
+Qed.
+
+Lemma field_offset_next_in_range: forall i m sz,
+  in_members i m ->
+  sizeof_struct cenv_cs 0 m <= sz ->
   field_offset cenv_cs i m + sizeof (field_type i m) <=
   field_offset_next cenv_cs i m sz <= sz.
 Proof.
   intros.
-  destruct m as [| m1 m]; [inversion H |].
-  unfold sizeof_struct in H0.
+  destruct m as [| [i0 t0] m]; [inversion H |].
   unfold field_offset, Ctypes.field_offset, field_offset_next, field_type.
-  pattern 0 at 4 5; replace 0 with (align (0*8) (alignof (type_member m1))) by (apply align_0, alignof_pos).
-  match goal with
-  | |- ?A => assert (A /\
-                     match field_offset_rec cenv_cs i (m1 :: m) 0 with
-                     | Errors.OK _ => True
-                     | _ => False
-                     end /\
-                     match Ctypes.field_type i (m1 :: m) with
-                     | Errors.OK _ => True
-                     | _ => False
-                     end); [| tauto]
-  end.
-  inv PLAIN. rename H4 into PLAIN. rename H3 into PLAIN1.
-  rewrite <- (Z.mul_0_l 8) in H0.
- change (field_offset_rec cenv_cs i (m1::m) 0) with (field_offset_rec cenv_cs i (m1::m) (0*8)).
-  revert m1 PLAIN1 H H0; generalize 0.
-  induction m as [| m0 m]; intros.
-  + destruct (ident_eq i (name_member m1)); [| destruct H; simpl in H; try congruence; tauto].
+  pattern 0 at 2 3; replace 0 with (align 0 (alignof t0)) by (apply align_0, alignof_pos).
+  revert i0 t0 H H0; generalize 0; induction m as [| [i1 t1] m]; intros.
+  + destruct (ident_eq i i0); [| destruct H; simpl in H; try congruence; tauto].
     subst; simpl.
-    rewrite !if_true by auto.
-    destruct m1; inv PLAIN1. simpl in *.
-    split; [| split]; auto.
-    unfold bitalignof, bitsizeof, bytes_of_bits in *.
-    split; [ | lia].
-    eapply Z.le_trans; try apply H0. clear H0.
-    rewrite <- (Z.div_mul (sizeof t) 8) by computable.
-    pose proof (sizeof_pos t).
-    fold (sizeof t). forget (sizeof t) as s.
-    pose proof (Ctypes.alignof_pos t).
-    forget (Ctypes.alignof t) as a. 
-     unfold align.
-    replace (z*8 + a*8 - 1) with ((z*8-1)+1*(a*8)) by lia.
-    rewrite Z.div_add by lia.
-    replace (((z * 8 - 1) / (a * 8) + 1) * (a * 8)  + s*8 + 7) with (((z * 8 - 1) / (a * 8) + 1) * (a * 8)  + 7 + s*8) by lia.
-    rewrite Z.div_add by lia.
-    rewrite Z.div_mul by lia.
-    apply Zplus_le_compat_r.
-    apply Z.div_le_mono. computable. lia.
-  + remember (m0::m) as m0'.  simpl in H0 |- *. subst m0'.
-     destruct m1; inv PLAIN1. simpl in *.
-     if_tac.
-    - split; [| split]; auto.
-      split.
+    if_tac; [| congruence].
+    simpl in H0.
+   fold (sizeof t0) in *.
+    lia.
+  + remember ((i1, t1) :: m) as m0. simpl in H0 |- *. subst m0.
+    destruct (ident_eq i i0).
+    - split.
       * apply align_le, alignof_pos.
       * pose proof sizeof_struct_incr cenv_cs m (align (align z (alignof t0) + sizeof t0)
             (alignof t1) + sizeof t1).
@@ -480,7 +631,6 @@ intros; subst.
 induction q; simpl; auto.
 Defined.
 
-
 (* copied from veric/Clight_lemmas.v; but here Defined instead of Qed  *)
 Lemma id_in_list_true: forall i ids, id_in_list i ids = true -> In i ids.
 Proof.
@@ -489,7 +639,6 @@ Proof.
  apply Pos_eqb_eq in Heqb. left; auto.
  auto.
 Defined.
-
 
 Lemma id_in_list_false: forall i ids, id_in_list i ids = false -> ~In i ids.
 Proof.
@@ -520,7 +669,7 @@ Proof.
       split; intros. split; auto. destruct H; auto.
 Defined.
 
-Lemma map_members_ext: forall A (f f':ident * type -> A) (m: members),
+Lemma map_members_ext: forall A (f f':ident * type -> A) (m: list (ident*type)),
   members_no_replicate m = true ->
   (forall i, in_members i m -> f (i, field_type i m) = f' (i, field_type i m)) ->
   map f m = map f' m.
@@ -609,13 +758,18 @@ Proof.
       auto.
 Qed.
 
+Lemma sizeof_union_pos:
+  forall env m, 0 <= sizeof_union env m.
+Proof.
+  induction m as [|[id t]]; simpl; extlia.
+Qed.
+
 Lemma sizeof_union_0: forall env i m,
   sizeof_union env m = 0 ->
   in_members i m ->
   Ctypes.sizeof (field_type i m) = 0.
 Proof.
   intros.
-  unfold field_type.
   induction m as [| (i0, t0) m].
   + inversion H0.
   + simpl in H.
@@ -676,12 +830,48 @@ Defined.
 
 End COMPOSITE_ENV.
 
-Lemma members_spec_change_composite' {cs_from cs_to} {CCE: change_composite_env cs_from cs_to}: forall id,
+Lemma members_spec_change_composite' {cs_from cs_to} {CCE: change_composite_env cs_from cs_to}: 
+  forall id m
+  (PLAIN: plain_members (co_members (@get_co cs_to id)) = Some m),
   match (coeq cs_from cs_to) ! id with
   | Some b => test_aux cs_from cs_to b id
   | None => false
   end = true ->
-  Forall (fun it => cs_preserve_type cs_from cs_to (coeq _ _) (snd it) = true) (co_members (get_co id)).
+  Forall (fun it => cs_preserve_type cs_from cs_to (coeq _ _) (snd it) = true) m.
+Proof.
+  intros.
+  destruct ((@cenv_cs cs_to) ! id) eqn:?H.
+  + pose proof proj1 (coeq_complete _ _ id) (ex_intro _ c H0) as [b ?].
+    rewrite H1 in H.
+    apply (coeq_consistent _ _ id _ _ H0) in H1.
+    unfold test_aux in H.
+    destruct b; [| inv H].
+    rewrite !H0 in H.
+    destruct ((@cenv_cs cs_from) ! id) eqn:?H; [| inv H].
+    simpl in H.
+    rewrite !andb_true_iff in H.
+    unfold get_co in PLAIN.
+    rewrite H0 in PLAIN.
+    clear - H1 PLAIN.
+    symmetry in H1.
+    revert m PLAIN; induction (co_members c) as [|[|]]; intros.
+    - inv PLAIN. constructor.
+    - simpl in PLAIN. destruct (plain_members m) eqn:?H; inv PLAIN.
+       simpl in H1; rewrite andb_true_iff in H1; destruct H1.
+      constructor; auto.
+    - inv PLAIN.
+  + destruct ((coeq cs_from cs_to) ! id) eqn:?H.
+    - pose proof proj2 (coeq_complete _ _ id) (ex_intro _ b H1) as [co ?].
+      congruence.
+    - inv H.
+Qed.
+
+Lemma members_spec_change_composite'delete_me {cs_from cs_to} {CCE: change_composite_env cs_from cs_to}: forall id,
+  match (coeq cs_from cs_to) ! id with
+  | Some b => test_aux cs_from cs_to b id
+  | None => false
+  end = true ->
+  Forall (fun m => cs_preserve_type cs_from cs_to (coeq _ _) (type_member m) = true) (co_members (@get_co cs_to id)).
 Proof.
   intros.
   destruct ((@cenv_cs cs_to) ! id) eqn:?H.
@@ -698,7 +888,7 @@ Proof.
     rewrite H0.
     clear - H1.
     symmetry in H1.
-    induction (co_members c) as [| [i t] ?].
+    induction (co_members c).
     - constructor.
     - simpl in H1; rewrite andb_true_iff in H1; destruct H1.
       constructor; auto.
@@ -708,39 +898,132 @@ Proof.
     - inv H.
 Qed.
 
-Lemma members_spec_change_composite'' {cs_from cs_to} {CCE: change_composite_env cs_from cs_to}: forall id,
+Lemma members_spec_change_composite'' {cs_from cs_to} {CCE: change_composite_env cs_from cs_to}:
+  forall id m
+  (PLAIN: plain_members (co_members (@get_co cs_to id)) = Some m),
   match (coeq cs_from cs_to) ! id with
   | Some b => test_aux cs_from cs_to b id
   | None => false
   end = true ->
-  forall i, cs_preserve_type cs_from cs_to (coeq _ _) (field_type i (co_members (get_co id))) = true.
+  forall i, cs_preserve_type cs_from cs_to (coeq _ _) (field_type i m) = true.
 Proof.
   intros.
-  unfold field_type.
-  apply members_spec_change_composite' in H.
-  induction H as [| [i0 t0] ?]; auto.
-  simpl.
-  if_tac; auto.
+  apply (@members_spec_change_composite' cs_from cs_to _ _ _ PLAIN) in H.
+  clear PLAIN.
+  induction H as [|[??]]; auto.
+  simpl; if_tac; auto.
 Qed.
 
-Lemma members_spec_change_composite {cs_from cs_to} {CCE: change_composite_env cs_from cs_to}: forall id,
+Definition field_type'' i m := match Ctypes.field_type i m with Errors.OK t => t | _ => Tvoid end.
+Lemma members_spec_change_composite''_delete_me {cs_from cs_to} {CCE: change_composite_env cs_from cs_to}: forall id,
   match (coeq cs_from cs_to) ! id with
   | Some b => test_aux cs_from cs_to b id
   | None => false
   end = true ->
-  Forall (fun it => cs_preserve_type cs_from cs_to (coeq _ _) (field_type (fst it) (co_members (get_co id))) = true) (co_members (get_co id)).
+  forall i, cs_preserve_type cs_from cs_to (coeq _ _) (field_type'' i (co_members (get_co id))) = true.
 Proof.
   intros.
-  apply members_spec_change_composite' in H.
-  assert (Forall (fun it: ident * type => field_type (fst it) (co_members (get_co id)) = snd it) (co_members (get_co id))).
+  unfold field_type''.
+  apply members_spec_change_composite'delete_me in H.
+  induction H as [|[|]]; auto;
+  simpl; if_tac; auto.
+Qed.
+
+Lemma plain_members_no_replicate:
+  forall {cs: compspecs} (id: positive) m, 
+    plain_members (co_members (get_co id)) = Some m ->
+    members_no_replicate m = true.
+Proof.
+ intros.
+ pose proof (get_co_members_no_replicate id).
+ unfold members_no_replicate.
+ unfold mpred.members_no_replicate in H0.
+ revert m H; induction (co_members (get_co id)) as [|[|]]; intros.
+ -
+ inv H. reflexivity.
+ -
+ simpl in *.
+ destruct (plain_members m) eqn:?H; inv H.
+ simpl.
+ destruct (id_in_list id0 (map fst l)) eqn:?H;
+ destruct (id_in_list id0 (map name_member m)) eqn:?H; auto.
+ clear - H2 H1 H.
+ revert l H1 H; induction m as [|[|]]; simpl; intros. inv H1. inv H.
+ destruct (plain_members m) eqn:?H; inv H1.
+ simpl map in H2,H.
+ unfold id_in_list in H2,H; fold id_in_list in H2,H.
+ rewrite orb_false_iff in H2.
+ rewrite orb_true_iff in H. destruct H2,H; try tauto; try congruence; eauto.
+ inv H1.
+ inv H0.
+ -
+  inv H.
+Qed.
+ 
+Lemma members_spec_change_composite {cs_from cs_to} {CCE: change_composite_env cs_from cs_to}:
+  forall id m
+  (PLAIN: plain_members (co_members (@get_co cs_to id)) = Some m),
+  match (coeq cs_from cs_to) ! id with
+  | Some b => test_aux cs_from cs_to b id
+  | None => false
+  end = true ->
+  Forall (fun it => cs_preserve_type cs_from cs_to (coeq _ _) (field_type (fst it) m) = true) m.
+Proof.
+  intros.
+  apply (members_spec_change_composite' _ _ PLAIN) in H.
+  assert (Forall (fun it: ident * type => field_type (fst it) m = snd it) m).
   1:{
     rewrite Forall_forall.
     intros it ?.
     apply In_field_type; auto.
-    apply get_co_members_no_replicate.
+    apply plain_members_no_replicate in PLAIN; auto.
+  }
+  revert H0.
+ clear PLAIN.
+ generalize m at 1 3.
+  induction H as [| [i t] ?]; constructor.
+  + inv H1.
+    simpl in *.
+    rewrite H4; auto.
+  + inv H1. 
+    auto.
+Qed.
+
+Lemma members_spec_change_composite_delete_me {cs_from cs_to} {CCE: change_composite_env cs_from cs_to}: forall id,
+  match (coeq cs_from cs_to) ! id with
+  | Some b => test_aux cs_from cs_to b id
+  | None => false
+  end = true ->
+  Forall (fun m => cs_preserve_type cs_from cs_to (coeq _ _) (field_type'' (name_member m) (co_members (get_co id))) = true) (co_members (get_co id)).
+Proof.
+  intros.
+  apply members_spec_change_composite'delete_me in H.
+  assert (Forall (fun m: member => field_type'' (name_member m) (co_members (get_co id)) = type_member m) (co_members (get_co id))).
+  1:{
+    rewrite Forall_forall.
+    intros it ?.
+    clear - H0.
+    pose proof (get_co_members_no_replicate id).
+    apply compute_list_norepet_e in H.
+    induction (co_members (get_co id)) as [|[|]]. inv H0. inv H.
+    -
+    unfold field_type''; simpl.
+    destruct H0. subst. 
+    if_tac. auto. simpl in H. contradiction.
+    if_tac. subst id0. contradiction H3. clear - H.
+    apply (in_map name_member) in H. auto.
+    apply IHm; auto. 
+    -
+    unfold field_type''; simpl.
+    destruct H0. subst. 
+    if_tac. auto. simpl in H. contradiction.
+    inv H.
+    if_tac. subst id0. contradiction H3. clear - H0.
+    apply (in_map name_member) in H0. auto.
+    apply IHm; auto. 
   }
   revert H0; generalize (co_members (get_co id)) at 1 3.
-  induction H as [| [i t] ?]; constructor.
+  induction H; constructor.
   + inv H1.
     simpl in *.
     rewrite H4; auto.
@@ -749,19 +1032,22 @@ Proof.
 Qed.
 
 (* TODO: we have already proved a related field_offset lemma in veric/change_compspecs.v. But it seems not clear how to use that in an elegant way. *)
-Lemma field_offset_change_composite {cs_from cs_to} {CCE: change_composite_env cs_from cs_to}: forall id i,
+Lemma field_offset_change_composite {cs_from cs_to} {CCE: change_composite_env cs_from cs_to}: 
+  forall id m
+  (PLAIN: plain_members (co_members (@get_co cs_to id)) = Some m)
+  i,
   match (coeq cs_from cs_to) ! id with
   | Some b => test_aux cs_from cs_to b id
   | None => false
   end = true ->
-  field_offset (@cenv_cs cs_from) i (co_members (@get_co cs_to id)) =
-  field_offset (@cenv_cs cs_to) i (co_members (@get_co cs_to id)).
+  field_offset (@cenv_cs cs_from) i m =
+  field_offset (@cenv_cs cs_to) i m.
 Proof.
   intros.
-  apply members_spec_change_composite' in H.
-  unfold field_offset, Ctypes.field_offset.
-  generalize 0 at 1 3.
-  induction (co_members (get_co id)) as [| [i0 t0] ?]; intros.
+  apply (members_spec_change_composite' _ _ PLAIN) in H. clear PLAIN.
+  unfold field_offset.
+  generalize 0.
+  induction m as [| [i0 t0] ?]; intros.
   + auto.
   + simpl.
     inv H.
@@ -775,17 +1061,20 @@ Proof.
       apply IHm.
 Qed.
 
-Lemma field_offset_next_change_composite {cs_from cs_to} {CCE: change_composite_env cs_from cs_to}: forall id i,
+Lemma field_offset_next_change_composite {cs_from cs_to} {CCE: change_composite_env cs_from cs_to}: 
+  forall id m
+  (PLAIN: plain_members (co_members (@get_co cs_to id)) = Some m)
+  i,
   match (coeq cs_from cs_to) ! id with
   | Some b => test_aux cs_from cs_to b id
   | None => false
   end = true ->
-  field_offset_next (@cenv_cs cs_from) i (co_members (get_co id)) (co_sizeof (@get_co cs_from id)) =
-field_offset_next (@cenv_cs cs_to) i (co_members (get_co id)) (co_sizeof (@get_co cs_to id)).
+  field_offset_next (@cenv_cs cs_from) i m (co_sizeof (@get_co cs_from id)) =
+  field_offset_next (@cenv_cs cs_to) i m (co_sizeof (@get_co cs_to id)).
 Proof.
   intros.
   rewrite co_sizeof_get_co_change_composite by auto.
-  apply members_spec_change_composite' in H.
+  apply (members_spec_change_composite' _ _ PLAIN) in H. clear PLAIN.
   unfold field_offset_next.
   generalize 0.
   destruct H as [| [i0 t0] ? ]; intros; auto.
